Capture/Grammar.lean
@@ -1,3 +1,4 @@
 import Capture.Grammar.Lang
-import Capture.Grammar.Start
 import Capture.Grammar.Grammar
+import Capture.Grammar.Capture
+import Capture.Grammar.Extract
