Capture/Grammar/Capture.lean
@@ -1,0 +1,281 @@
+import Capture.Regex.Regex
+import Capture.Grammar.Grammar
+import Capture.Grammar.Extract
+
+import Capture.Std.Hedge
+
+def neutralize (x: Regex (φ × Ref n) α): Regex (φ × Ref n) α :=
+  match x with
+  | Regex.emptyset => Regex.emptyset
+  | Regex.emptystr => Regex.emptystr
+  | Regex.matched a => Regex.matched a
+  | Regex.symbol _ => Regex.emptyset
+  | Regex.or y z => Regex.or (neutralize y) (neutralize z)
+  | Regex.concat y z => Regex.concat (neutralize y) (neutralize z)
+  | Regex.star y => Regex.star (neutralize y)
+  | Regex.group id y => Regex.group id (neutralize y)
+
+partial def derive (G: Grammar n φ (Captured α)) (Φ: φ -> α -> Bool) (x: Regex (φ × Ref n) (Captured α)) (node: Hedge.Node α): Regex (φ × Ref n) (Captured α) :=
+  match x with
+  | Regex.emptyset => Regex.emptyset
+  | Regex.emptystr => Regex.emptyset
+  -- remember matched is just epsilon, so has the same derivative.
+  | Regex.matched _ => Regex.emptyset
+  | Regex.symbol (labelPred, ref) =>
+    match node with
+    | Hedge.Node.mk label children =>
+      if Φ labelPred label
+      then
+        let dchild := List.foldl (derive G Φ) (G.lookup ref) children
+        if dchild.null
+        then Regex.matched (label, extract dchild)
+        else Regex.emptyset
+      else Regex.emptyset
+  | Regex.or y z => Regex.or (derive G Φ y node) (derive G Φ z node)
+  | Regex.concat y z =>
+    if Regex.null y
+    then Regex.or
+      (Regex.concat (derive G Φ y node) z)
+      -- A difference from the usual derive algorithm:
+      -- To preserve the capture information in the nullable expression y,
+      -- instead of (derive z node), we write:
+      (Regex.concat (neutralize y) (derive G Φ z node))
+    else Regex.concat (derive G Φ y node) z
+  | Regex.star y => Regex.concat (derive G Φ y node) x
+  | Regex.group n y =>
+    Regex.group n (derive G Φ y node)
+
+
+def captures (G: Grammar n φ (Captured α)) (Φ: φ -> α -> Bool) (x: Regex (φ × Ref n) (Captured α)) (nodes: Hedge α): Option (List (Nat × Hedge α)) :=
+  let dx := List.foldl (derive G Φ) x nodes
+  if dx.null
+  then Option.some (extractGroups dx)
+  else Option.none
+
+def capture [Ord α] (G: Grammar n φ (Captured α)) (Φ: φ -> α -> Bool) (name: Nat) (x: Regex (φ × Ref n) (Captured α)) (nodes: Hedge α): Option (Hedge α) :=
+  match captures G Φ x nodes with
+  | Option.none => Option.none
+  | Option.some cs =>
+  let hedges := List.filterMap
+    (fun (name', forest) =>
+      if name = name'
+      then Option.some forest
+      else Option.none
+    ) cs
+  List.head? (List.reverse (List.mergeSort hedges (le := fun x y => (Ord.compare x y).isLE)))
+
+-- capturePaths is just like captures, except extractGroups is replaced by extractPathGroups
+def capturePaths (G: Grammar n φ (Captured α)) (Φ: φ -> α -> Bool) (x: Regex (φ × Ref n) (Captured α)) (forest: Hedge α): Option (List (Nat × Hedge α)) :=
+  let dx := List.foldl (derive G Φ) x forest
+  if dx.null
+  then Option.some (extractPathGroups dx)
+  else Option.none
+
+-- capturePath is just like capture, except captures is replaced by capturePaths
+def capturePath [Ord α] (G: Grammar n φ (Captured α)) (Φ: φ -> α -> Bool) (name: Nat) (x: Regex (φ × Ref n) (Captured α)) (forest: Hedge α): Option (Hedge α) :=
+  match capturePaths G Φ x forest with
+  | Option.none => Option.none
+  | Option.some cs =>
+  let forests := List.filterMap
+    (fun (name', forest) =>
+      if name = name'
+      then Option.some forest
+      else Option.none
+    ) cs
+  List.head? (List.reverse (List.mergeSort forests (le := fun x y => (Ord.compare x y).isLE)))
+
+def Regex.char (c: Char): Regex (Char × Ref (n + 1)) (Captured Char) :=
+  Regex.symbol (c, 0)
+
+instance {α : Type u} [DecidableEq α] : DecidableEq (Option α) := inferInstance
+
+def treeString (s: String): Hedge Char :=
+  List.map (fun c => Hedge.Node.mk c []) s.toList
+
+def runCaptures (G: Grammar n Char (Captured Char)) (xs: Hedge Char): Option (List (Nat × Hedge Char)) :=
+  captures G (· == ·) G.start xs
+
+def runCapture (id: Nat) (G: Grammar n Char (Captured Char)) (xs: Hedge Char): Option (Hedge Char) :=
+  capture G (· == ·) id G.start xs
+
+def runCapturePath (id: Nat) (G: Grammar n Char (Captured Char)) (xs: Hedge Char): Option (Hedge Char) :=
+  capturePath G (· == ·) id G.start xs
+
+-- no group
+#guard runCaptures
+  (Grammar.mk (Regex.char 'a') #v[Regex.emptystr])
+  (treeString "a")
+  == Option.some []
+
+-- simplest group
+#guard runCaptures
+  (Grammar.mk (Regex.group 1 (Regex.char 'a')) #v[Regex.emptystr])
+  (treeString "a")
+  == Option.some [(1, [Hedge.Node.mk 'a' []])]
+
+#guard runCapture 1 (Grammar.mk (Regex.concat (Regex.concat
+    (Regex.star (Regex.char 'a'))
+    (Regex.group 1 (Regex.char 'b')))
+    (Regex.star (Regex.char 'a'))
+  ) #v[Regex.emptystr])
+  (treeString "aaabaaa")
+  == Option.some (treeString "b")
+
+
+#guard runCapture 1 (Grammar.mk (Regex.concat (Regex.concat
+    (Regex.star (Regex.char 'a'))
+    (Regex.group 1 (Regex.star (Regex.char 'b'))))
+    (Regex.star (Regex.char 'a'))
+  ) #v[Regex.emptystr])
+  (treeString "aaabbbaaa")
+  == Option.some (treeString "bbb")
+
+#guard runCapture 1 (Grammar.mk (Regex.concat (Regex.concat
+    (Regex.star (Regex.char 'a'))
+    (Regex.group 1
+      (Regex.or
+        (Regex.star (Regex.char 'b'))
+        (Regex.star (Regex.char 'c'))
+      )
+    ))
+    (Regex.star (Regex.char 'a'))
+  ) #v[Regex.emptystr])
+  (treeString "aaacccaaa")
+  == Option.some (treeString "ccc")
+
+#guard runCapture 1 (Grammar.mk (Regex.concat (Regex.concat
+    (Regex.star (Regex.char 'a'))
+    (Regex.group 1
+      (Regex.or
+        (Regex.star (Regex.char 'b'))
+        (Regex.concat (Regex.char 'b') (Regex.star (Regex.char 'c')))
+      )
+    ))
+    (Regex.star (Regex.char 'a'))
+  ) #v[Regex.emptystr])
+  (treeString "aaabccaaa")
+  == Option.some (treeString "bcc")
+
+#guard runCapture 1 (Grammar.mk (Regex.concat (Regex.concat
+    (Regex.star (Regex.char 'a'))
+    (Regex.group 1 (Regex.char 'b')))
+    (Regex.star (Regex.char 'a'))
+  ) #v[Regex.emptystr])
+  [
+    Hedge.Node.mk 'a' [],
+    Hedge.Node.mk 'a' [],
+    Hedge.Node.mk 'a' [],
+    Hedge.Node.mk 'b' [],
+    Hedge.Node.mk 'a' [],
+    Hedge.Node.mk 'a' [],
+    Hedge.Node.mk 'a' []
+  ]
+  == Option.some [
+    Hedge.Node.mk 'b' []
+  ]
+
+#guard runCapture 1 (Grammar.mk (Regex.group 1 (Regex.symbol ('b', 1)))
+    #v[Regex.emptystr, (Regex.char 'c')]
+  )
+  [
+    Hedge.Node.mk 'b' [
+      Hedge.Node.mk 'c' [],
+    ],
+  ]
+  == Option.some [
+    Hedge.Node.mk 'b' [
+      Hedge.Node.mk 'c' []
+    ]
+  ]
+
+#guard runCapture 1
+  (Grammar.mk (Regex.symbol ('b', 1)) #v[Regex.emptystr, Regex.group 1 (Regex.char 'c')])
+  [
+    Hedge.Node.mk 'b' [
+      Hedge.Node.mk 'c' [],
+    ],
+  ]
+  == Option.some [
+    Hedge.Node.mk 'c' []
+  ]
+
+#guard runCapturePath 1
+  (Grammar.mk (Regex.symbol ('b', 1)) #v[Regex.emptystr, Regex.group 1 (Regex.char 'c')])
+  [
+    Hedge.Node.mk 'b' [
+      Hedge.Node.mk 'c' [],
+    ],
+  ]
+  == Option.some [
+    Hedge.Node.mk 'b' [
+      Hedge.Node.mk 'c' []
+    ]
+  ]
+
+#guard runCapture 1
+  (Grammar.mk (Regex.concat (Regex.concat
+    (Regex.star (Regex.char 'a'))
+    (Regex.symbol ('b', 1)))
+    (Regex.star (Regex.char 'a'))
+  )
+  #v[Regex.emptystr, (Regex.concat (Regex.concat
+        (Regex.star (Regex.char 'a'))
+        (Regex.group 1 (Regex.char 'c')))
+        (Regex.star (Regex.char 'a')))
+    ]
+  )
+  [
+    Hedge.Node.mk 'a' [],
+    Hedge.Node.mk 'a' [],
+    Hedge.Node.mk 'a' [],
+    Hedge.Node.mk 'b' [
+      Hedge.Node.mk 'a' [],
+      Hedge.Node.mk 'a' [],
+      Hedge.Node.mk 'a' [],
+      Hedge.Node.mk 'c' [],
+      Hedge.Node.mk 'a' [],
+      Hedge.Node.mk 'a' [],
+      Hedge.Node.mk 'a' [],
+    ],
+    Hedge.Node.mk 'a' [],
+    Hedge.Node.mk 'a' [],
+    Hedge.Node.mk 'a' []
+  ]
+  == Option.some [
+    Hedge.Node.mk 'c' []
+  ]
+
+#guard runCapturePath 1
+  (Grammar.mk (Regex.concat (Regex.concat
+    (Regex.star (Regex.char 'a'))
+    (Regex.symbol ('b', 1)))
+    (Regex.star (Regex.char 'a'))
+  )
+  #v[Regex.emptystr, (Regex.concat (Regex.concat
+        (Regex.star (Regex.char 'a'))
+        (Regex.group 1 (Regex.char 'c')))
+        (Regex.star (Regex.char 'a')))
+    ]
+  )
+  [
+    Hedge.Node.mk 'a' [],
+    Hedge.Node.mk 'a' [],
+    Hedge.Node.mk 'a' [],
+    Hedge.Node.mk 'b' [
+      Hedge.Node.mk 'a' [],
+      Hedge.Node.mk 'a' [],
+      Hedge.Node.mk 'a' [],
+      Hedge.Node.mk 'c' [],
+      Hedge.Node.mk 'a' [],
+      Hedge.Node.mk 'a' [],
+      Hedge.Node.mk 'a' [],
+    ],
+    Hedge.Node.mk 'a' [],
+    Hedge.Node.mk 'a' [],
+    Hedge.Node.mk 'a' []
+  ]
+  == Option.some [
+    Hedge.Node.mk 'b' [
+      Hedge.Node.mk 'c' []
+    ]
+  ]
