Capture/Grammar/Extract.lean
@@ -1,0 +1,56 @@
+import Capture.Regex.Regex
+import Capture.Grammar.Grammar
+
+import Capture.Std.Hedge
+
+
+def extract (x: Regex σ (Captured α)): Hedge (Nat ⊕ α) :=
+  match x with
+  -- should never be encountered, since emptyset is not nullable.
+  | Regex.emptyset => []
+  | Regex.emptystr => []
+  -- should never be encountered, since tree is not nullable.
+  | Regex.symbol _ => []
+  | Regex.matched (label, captured) => [Hedge.Node.mk (Sum.inr label) captured]
+  | Regex.or y z =>
+    -- Under POSIX semantics, we prefer matching the left alternative.
+    if y.null
+    then extract y
+    else extract z
+  | Regex.concat y z =>
+    extract y ++ extract z
+    -- Groups under a star are ignored.
+    -- Recursively extracting under the star causes empty captures to be reported, which we do not want under POSIX semantics.
+  | Regex.star _ => []
+    -- Ignore group, this group will be extracted later by extractGroups.
+  | Regex.group n y => [Hedge.Node.mk (Sum.inl n) (extract y)]
+
+def extractHedge (xs: Hedge (Nat ⊕ α)): Hedge α :=
+  match xs with
+  | [] => []
+  | Hedge.Node.mk (Sum.inl _id) children::xs' =>
+    extractHedge children ++ extractHedge xs'
+  | Hedge.Node.mk (Sum.inr a) children::xs' =>
+    Hedge.Node.mk a (extractHedge children)::extractHedge xs'
+
+def extractGroups' (xs: Hedge (Nat ⊕ α)): List (Nat × Hedge α) :=
+  match xs with
+  | [] => []
+  | Hedge.Node.mk (Sum.inl id) children::xs' =>
+    (id, extractHedge children) :: extractGroups' xs'
+  | Hedge.Node.mk (Sum.inr _a) children::xs' =>
+    extractGroups' children ++ extractGroups' xs'
+
+def extractPathGroups' (xs: Hedge (Nat ⊕ α)): List (Nat × Hedge α) :=
+  match xs with
+  | [] => []
+  | Hedge.Node.mk (Sum.inl id) children::xs' =>
+    (id, extractHedge children) :: extractPathGroups' xs'
+  | Hedge.Node.mk (Sum.inr a) children::xs' =>
+    List.map (fun (id, h) => (id, [Hedge.Node.mk a h])) (extractPathGroups' children) ++ extractPathGroups' xs'
+
+def extractGroups (x: Regex σ (Captured α)): List (Nat × Hedge α) :=
+  extractGroups' (extract x)
+
+def extractPathGroups (x: Regex σ (Captured α)): List (Nat × Hedge α) :=
+  extractPathGroups' (extract x)
