Capture/Regex/Map.lean
@@ -3,10 +3,10 @@
 
 import Capture.Regex.Regex
 
-def Regex.map (r: Regex α) (f: α → β): Regex β := match r with
+def Regex.map (r: Regex σ₁ α) (f: σ₁ → σ₂): Regex σ₂ α := match r with
   | emptyset => emptyset
   | emptystr => emptystr
-  | matched s => matched (f s)
+  | matched a => matched a
   | symbol s => symbol (f s)
   | or r1 r2 => or (map r1 f) (map r2 f)
   | concat r1 r2 => concat (map r1 f) (map r2 f)
@@ -15,7 +15,7 @@ def Regex.map (r: Regex α) (f: α → β): Regex β := match r with
 
 namespace Regex
 
-theorem map_id (r: Regex α):
+theorem map_id (r: Regex σ₁ α):
   map r (fun s => s) = r := by
   induction r with
   | emptyset =>
@@ -41,7 +41,7 @@ theorem map_id (r: Regex α):
     simp only [map]
     rw [ih1]
 
-theorem map_map (r: Regex α) (f: α → β) (g: β → σ):
+theorem map_map (r: Regex σ₁ α) (f: σ₁ → σ₂) (g: σ₂ → σ₃):
   map (map r f) g = map r (fun r' => g (f r')) := by
   induction r with
   | emptyset =>
@@ -67,7 +67,7 @@ theorem map_map (r: Regex α) (f: α → β) (g: β → σ):
     simp only [map]
     rw [ih1]
 
-theorem map_null {σ} (Φ: σ → Bool) (r: Regex σ):
+theorem map_null {σ} (Φ: σ → Bool) (r: Regex σ α):
   (map r (fun s => (s, Φ s))).null = r.null := by
   induction r with
   | emptyset =>
@@ -91,21 +91,3 @@ theorem map_null {σ} (Φ: σ → Bool) (r: Regex σ):
   | group _ r1 ih1 =>
     simp only [map, Regex.null]
     rw [ih1]
-
-instance: Functor Regex where
-  map f := Regex.map (f := f)
-
-instance: LawfulFunctor Regex where
-  map_const {α β}: (Functor.mapConst : α → Regex β → Regex α) = Functor.map ∘ Function.const β := by
-    unfold Functor.mapConst
-    unfold instFunctor
-    unfold Function.const
-    unfold Functor.map
-    simp only
-  id_map {α} (x : Regex α) : id <$> x = x := by apply map_id
-  comp_map {α β γ} (f : α → β) (g : β → γ) (r : Regex α) : (g ∘ f) <$> r = g <$> f <$> r := by
-    unfold Functor.map
-    unfold instFunctor
-    simp only
-    rw [map_map]
-    rfl
